## [10. Regular Expression Matching](https://leetcode.cn/problems/regular-expression-matching/)

### First Solution
**Java**
```java
class Solution {
    public boolean isMatch(String s, String p) {
        int n = s.length(),  m = p.length();
        boolean[][] dp = new boolean[n + 1][m + 1];
        dp[0][0] = true;
        for(int i = 1; i < n; i += 1) {
            dp[i][0] = false;
        }
        for(int j = 1; j <= m; j += 1) {
            if(p.charAt(j - 1) == '*') {
                dp[0][j] = dp[0][j - 2];
            }
        }
        for(int i = 1; i <= n; i += 1) {
            for(int j = 1; j <= m; j += 1) {
                char curS = s.charAt(i - 1), curP = p.charAt(j - 1);
                if(curS == curP || curP == '.') {
                    dp[i][j] = dp[i - 1][j - 1];
                } else if(curP == '*') {
                    char preP = p.charAt(j - 2);
                    if(curS == preP || preP == '.') {
                        // dp[i][j - 2]: p[j - 2] does not exist
                        // dp[i - 1][j - 2]: p[j - 2] exist once
                        // dp[i - ][j]: p[j - 2] exist more than once
                        dp[i][j] = dp[i][j - 2] || dp[i - 1][j - 2] || dp[i - 1][j];
                    } else {
                        dp[i][j] = dp[i][j - 2];
                    }
                }
            }
        }
        return dp[n][m];
    }
}
```
**Python**
```python
class Solution:
    def isMatch(self, s: str, p: str) -> bool:
        n, m = len(s), len(p)
        dp = [[False] * (m + 1) for _ in range(n + 1)]
        dp[0][0] = True
        for i in range(1, n + 1):
            dp[i][0] = False
        for j in range(1, m + 1):
            if p[j - 1] == '*':
                dp[0][j] = dp[0][j - 2]
        for i in range(1, n + 1):
            for j in range(1, m + 1):
                if s[i - 1] == p[j - 1] or p[j - 1] == '.':
                    dp[i][j] = dp[i - 1][j - 1]
                elif p[j - 1] == '*':
                    if s[i - 1] == p[j - 2] or p[j - 2] == '.':
                        dp[i][j] = dp[i][j - 2] or dp[i - 1][j - 2] or dp[i - 1][j]
                    else:
                        dp[i][j] = dp[i][j - 2]
        return dp[n][m]
```

|time complexity|space complexity|
|:-:|:-:|
|$O(n*m)$|$O(n*m)$|
where $n$ is the length of String s, $m$ is the length of String p