## [450. Delete Node in a BST](https://leetcode.cn/problems/delete-node-in-a-bst/)

### First Solution

**Java**
```java
class Solution {

    int sum = 0;

    public TreeNode convertBST(TreeNode root) {
        if(root == null) {
            return null;
        }
        root.right = convertBST(root.right);
        root.val += sum;
        sum = root.val;
        root.left = convertBST(root.left);
        return root;
    }
}
```
**Python**
```python
class Solution:
    def convertBST(self, root: Optional[TreeNode]) -> Optional[TreeNode]:
        sum = 0
        def helper(root):
            nonlocal sum
            if root is None:
                return None
            root.right = helper(root.right)

            root.val += sum
            sum = root.val

            root.left = helper(root.left)
            return root
        return helper(root)
```

### Second Solution

**Java**
```java
class Solution {

    public TreeNode convertBST(TreeNode root) {
        if(root == null) {
            return null;
        }
        TreeNode cur = root;
        int sum = 0;
        while(cur != null) {
            if(cur.right == null) {
                cur.val += sum;
                sum = cur.val;
                cur = cur.left;
                continue;
            } 
            TreeNode next = cur.right;
            while(next.left != null && next.left != cur) {
                next = next.left;
            }
            if(next.left == null) { // first reach
                next.left = cur;
                cur = cur.right;
            } else {
                cur.val += sum;
                sum = cur.val;
                next.left = null;
                cur = cur.left;
            }
        }
        return root;
    }
}
```
**Python**
```python
class Solution:
    def convertBST(self, root: Optional[TreeNode]) -> Optional[TreeNode]:
        if root is None:
            return None
        cur, sum = root, 0
        while cur:
            if cur.right is None:
                cur.val += sum
                sum = cur.val
                cur = cur.left
                continue
            next = cur.right
            while next.left and next.left != cur:
                next = next.left
            if next.left is None:
                next.left = cur
                cur = cur.right
            else:
                cur.val += sum
                sum = cur.val
                next.left = None
                cur = cur.left            
        return root
```
| time complexity | space complexity |
| :-------------: | :--------------: |
| $O(n)$          | $O(1)$           |